src/simple-proof/proof/Helper_lemmas.v
@@ -12,7 +12,121 @@ Require Import LibLN.
 Require Import Coq.Program.Equality.
 Require Import Definitions.
 
+(** [Gamma |- ds :: Ds]                     #<br>#
+    [Ds] is a record type with labels [ls] #<br>#
+    [ds] are definitions with label [ls']  #<br>#
+    [l notin ls']
+    --------------------------------------
+    [l notin ls] *)
+Lemma hasnt_notin : forall G ds ls l U,
+    G /- ds :: U ->
+    record_typ U ls ->
+    defs_hasnt ds l ->
+    l \notin ls.
+Proof.
+  introv Hds Hrec Hhasnt.
+  inversions Hhasnt. gen ds. induction Hrec; intros.
+  - inversions Hds. inversions H5; simpl in *; case_if; apply* notin_singleton.
+  - apply notin_union; split.
+    + inversions Hds. apply (IHHrec ds0 H5). simpl in *. case_if*.
+    + inversions Hds. inversions H8; simpl in *; case_if; apply* notin_singleton.
+Qed.
+
 (** * Lemmas About Opening *)
+
+(** The following [open_fresh_XYZ_injective] lemmas state that given two
+    symbols (variables, types, terms, etc.) [X] and [Y] and a variable [z],
+    if [z notin fv(X)] and [z notin fv(Y)], then [X^z = Y^z] entails [X = Y]. *)
+
+(** - opening of variables with fresh variables is injective. *)
+Lemma open_fresh_avar_injective : forall x y k z,
+    z \notin fv_avar x ->
+    z \notin fv_avar y ->
+    open_rec_avar k z x = open_rec_avar k z y ->
+    x = y.
+Proof.
+  intros. destruct x, y; inversion H1.
+  - case_if.
+    + case_if. subst. reflexivity.
+    + case_if. assumption.
+  - case_if. simpl in H0. inversions H3. false* notin_same.
+  - case_if. simpl in H. inversions H3. false* notin_same.
+  - reflexivity.
+Qed.
+
+(** - opening of types and declarations with fresh variables is injective. *)
+Lemma open_fresh_typ_dec_injective:
+  (forall T T' k x,
+    x \notin fv_typ T ->
+    x \notin fv_typ T' ->
+    open_rec_typ k x T = open_rec_typ k x T' ->
+    T = T') /\
+  (forall D D' k x,
+    x \notin fv_dec D ->
+    x \notin fv_dec D' ->
+    open_rec_dec k x D = open_rec_dec k x D' ->
+    D = D').
+Proof.
+  apply typ_mutind; intros.
+  - destruct T'; inversions H1. reflexivity.
+  - destruct T'; inversions H1. reflexivity.
+  - destruct T'; inversions H2. apply f_equal. apply* (H d0 k x).
+  - destruct T'; inversions H3.
+    assert (t = T'1). {
+      apply (H T'1 k x).
+      - simpl in H1. auto.
+      - simpl in H2. auto.
+      - assumption.
+    }
+    assert (t0 = T'2). {
+      apply (H0 T'2 k x).
+      - simpl in H1. auto.
+      - simpl in H2. auto.
+      - assumption.
+    }
+    subst*.
+  - destruct T'; inversions H1.
+    simpl in H. simpl in H0. pose proof (open_fresh_avar_injective a a0 k H H0 H3).
+    subst*.
+  - destruct T'; inversions H2.
+    apply f_equal. apply (H T' (Datatypes.S k) x).
+    + simpl in H. assumption.
+    + simpl in H0. assumption.
+    + assumption.
+  - destruct T'; inversions H3.
+    assert (t = T'1). {
+      apply (H T'1 k x).
+      - simpl in H1. auto.
+      - simpl in H2. auto.
+      - assumption.
+    }
+    assert (t0 = T'2). {
+      apply (H0 T'2 (S k) x).
+      - simpl in H1. auto.
+      - simpl in H2. auto.
+      - assumption.
+    }
+    subst*.
+  - destruct D'; inversions H3.
+    assert (t0 = t3). {
+      apply (H t3 k x).
+      - simpl in H1. auto.
+      - simpl in H2. auto.
+      - assumption.
+    }
+    assert (t1 = t4). {
+      apply (H0 t4 k x).
+      - simpl in H1. auto.
+      - simpl in H2. auto.
+      - assumption.
+    }
+    subst*.
+  - destruct D'; inversions H2.
+    apply f_equal. apply (H t2 k x).
+    + simpl in H0. assumption.
+    + simpl in H1. assumption.
+    + assumption.
+Qed.
 
 (** The following [open_comm_XYZ] lemmas state that opening two
     symbols (variables, types, terms, etc.) at different indices commute. *)
@@ -302,6 +416,79 @@ Lemma open_record_type: forall T x,
 Proof.
   intros. destruct H as [ls H]. exists ls. eapply open_record_typ.
   eassumption.
+Qed.
+
+(** The type of definitions is a record type. *)
+Lemma ty_defs_record_type : forall G ds T,
+    G /- ds :: T ->
+    record_type T.
+Proof.
+  intros.
+  dependent induction H.
+  - destruct D.
+    + inversions H. exists \{ label_typ t }. constructor*. constructor.
+    + exists \{ label_trm t }. constructor*. constructor.
+  - destruct IHty_defs. destruct D.
+    + exists (x \u \{ label_typ t }). constructor*.
+      * inversions H0. constructor.
+      * inversions H0. simpl in H1. apply (hasnt_notin H H2 H1).
+    + exists (x \u \{ label_trm t }). constructor*.
+      * constructor.
+      * inversions H0. simpl in H1. apply (hasnt_notin H H2 H1).
+Qed.
+
+
+(** Opening does not affect the labels of a [record_typ]. *)
+Lemma opening_preserves_labels : forall z T ls ls',
+    record_typ T ls ->
+    record_typ (open_typ z T) ls' ->
+    ls = ls'.
+Proof.
+  introv Ht Hopen. gen ls'.
+  dependent induction Ht; intros.
+  - inversions Hopen. rewrite* <- open_dec_preserves_label.
+  - inversions Hopen. rewrite* <- open_dec_preserves_label.
+    specialize (IHHt ls0 H4). rewrite* IHHt.
+Qed.
+
+(** Opening does not affect the labels of a [record_type]. *)
+Lemma record_type_open : forall z T,
+    z \notin fv_typ T ->
+    record_type (open_typ z T) ->
+    record_type T.
+Proof.
+  introv Hz H. destruct H. dependent induction H.
+  - exists \{ l }. destruct T; inversions x. constructor.
+    + destruct d; inversions H.
+      * apply (proj21 open_fresh_typ_dec_injective) in H3.
+        { subst. constructor. }
+        { simpl in Hz; auto. }
+        { simpl in Hz; auto. }
+      * constructor.
+    + destruct d; inversions H.
+      * apply (proj21 open_fresh_typ_dec_injective) in H3.
+        { subst. constructor. }
+        { simpl in Hz; auto. }
+        { simpl in Hz; auto. }
+      * constructor.
+  - destruct T; inversions x. simpl in Hz.
+    assert (Hz': z \notin fv_typ T1) by auto.
+    destruct (IHrecord_typ T1 z Hz' eq_refl) as [ls' ?]. clear Hz'.
+    destruct T2; inversions H5.
+    destruct d; inversions H0.
+    + exists (ls' \u \{ label_typ t }). apply (proj21 open_fresh_typ_dec_injective) in H6.
+      * subst. constructor*.
+        { constructor. }
+        {
+          simpl in H2. pose proof (opening_preserves_labels z H1 H).
+          rewrite* H0.
+        }
+      * simpl in Hz; auto.
+      * simpl in Hz; auto.
+    + exists (ls' \u \{ label_trm t }). constructor*.
+      * constructor.
+      * simpl in H2. pose proof (opening_preserves_labels z H1 H).
+        rewrite* H0.
 Qed.
 
 (** If [T] is a record type with labels [ls], and [T = ... /\ D /\ ...],
