src/simple-proof/proof/Precise_types.v
@@ -69,6 +69,18 @@ Proof.
     specialize (IHHpf S T eq_refl); inversion IHHpf.
 Qed.
 
+(** The precise type of a value is inert. *)
+Lemma precise_inert_typ : forall G v T,
+    G |-! trm_val v : T ->
+    inert_typ T.
+Proof.
+  introv Ht. inversions Ht; constructor; rename T0 into T.
+  pick_fresh z. assert (Hz: z \notin L) by auto. specialize (H1 z Hz).
+  pose proof (ty_defs_record_type H1).
+  assert (Hz': z \notin fv_typ T) by auto.
+  apply (record_type_open T Hz' H).
+Qed.
+
 (** The following two lemmas say that the type to which a variable is bound in an inert context is inert. *)
 Lemma binds_inert : forall G x T,
     binds x T G ->
