src/simple-proof/proof/Safety.v
@@ -102,19 +102,18 @@ Qed.
 Lemma preservation_hole: forall G s t e' t' T,
     lc_term (e_hole s) t ->
     e_hole s / t |-> e' / t' ->
-    inert G ->
     ty_ec_trm G (e_hole s) t T ->
-    exists G',
-      ty_ec_trm (G & G') e' t' T.
+    exists G', ty_ec_trm (G & G') e' t' T.
 Proof.
-  introv Hlc Hred Hin Ht.
-  inversions Ht. rename H0 into Hwf. rename H2 into Ht.
+  introv Hlc Hred Ht.
+  inversions Ht.
+  rename H0 into Hin. rename H1 into Hwf. rename H3 into Ht.
   lets Hlc': (red_preserves_lc Hred Hlc).
   dependent induction Ht; try solve [inversion Hred].
   - destruct (canonical_forms_fun Hin Hwf Ht1) as [L [T' [t [Bis [Hsub Hty]]]]].
     inversions Hred.
     apply (binds_func H4) in Bis. inversions Bis.
-    exists (@empty typ). rewrite concat_empty_r. repeat split; auto.
+    exists (@empty typ). rewrite concat_empty_r.
     pick_fresh y. assert (y \notin L) as FrL by auto. specialize (Hty y FrL).
     constructor*. rewrite subst_intro_typ with (x:=y); auto.
     rewrite subst_intro_trm with (x:=y); auto.
@@ -132,21 +131,20 @@ Proof.
     + eapply ty_e_hole; auto.
       apply weaken_subtyp with (G2:=G') in H; eauto.
     + apply_fresh ty_e_term as z; eauto; intros. assert (z \notin L) by auto.
-      specialize (H2 z H3).
+      specialize (H3 z H4).
       apply weaken_subtyp with (G2:=(G' & z ~ T0)) in H; rewrite concat_assoc in *; eauto.
 Qed.
 
 Lemma preservation: forall G e t e' t' T,
-    inert G ->
     lc_term e t ->
     e / t |-> e' / t' ->
     ty_ec_trm G e t T ->
     exists G', ty_ec_trm (G & G') e' t' T.
 Proof.
-  introv Hi Hlc Hred Ht.
+  introv Hlc Hred Ht.
+  inversions Ht; rename H into Hin; rename H0 into Hwf; rename H1 into Ht.
   inversion Hlc as [Hlc_ec Hlc_trm].
-  inversions Ht. apply* preservation_hole. constructor~.
-  rename H into Hwf. rename H0 into Ht.
+  apply* preservation_hole. constructor~.
   destruct t.
   - inversions Hred.
     pick_fresh y.
@@ -159,9 +157,10 @@ Proof.
     pose proof (wf_sto_notin_dom Hwf H5).
     pose proof (val_typing Ht) as [V [Hv Hs]].
     pick_fresh y. assert (y \notin L) by auto.
-    specialize (H1 y H0).
+    specialize (H2 y H0).
     exists (x ~ V).
     apply ty_e_hole.
+    * constructor~. eapply precise_inert_typ; eauto.
     * constructor~.
       apply (precise_to_general Hv).
     * rewrite subst_intro_trm with (x:=y); auto.
@@ -172,20 +171,20 @@ Proof.
       {
         rewrite~ subst_fresh_typ.
         pose proof (ty_var (binds_tail x V G)).
-        apply (ty_sub H2). apply (weaken_subtyp Hs); eauto.
+        apply (ty_sub H1). apply (weaken_subtyp Hs); eauto.
       }
   - inversion Hred. rewrite <- H4 in Hred. apply red_term_to_hole in Hred. subst.
     apply lc_term_to_hole in Hlc.
-    pose proof (preservation_hole Hlc Hred Hi (ty_e_hole Hwf Ht)) as [G' Ht'].
+    pose proof (preservation_hole Hlc Hred (ty_e_hole Hin Hwf Ht)) as [G' Ht'].
     inversions Ht'. exists G'.
     eapply ty_e_term with (L:=L \u (dom G) \u (dom G')); eauto. intros.
     assert (x0 \notin L) by auto.
-    specialize (H1 x0 H2).
+    specialize (H2 x0 H4).
     eapply (proj41 weaken_rules); eauto.
-  - inversion Hred. rewrite <- H2 in Hred.
+  - inversion Hred. rewrite <- H1 in Hred.
     apply red_term_to_hole in Hred. subst.
     apply lc_term_to_hole in Hlc.
-    pose proof (preservation_hole Hlc Hred Hi (ty_e_hole Hwf Ht)) as [G' Ht'].
+    pose proof (preservation_hole Hlc Hred (ty_e_hole Hin Hwf Ht)) as [G' Ht'].
     inversions Ht'. exists G'.
     eapply ty_e_term with (L:=L \u (dom G) \u (dom G')); eauto. intros.
     eapply (proj41 weaken_rules); eauto.
@@ -199,56 +198,56 @@ Proof.
       apply_fresh ty_let as z; eauto.
       unfold open_trm.
       rewrite~ (proj41 (open_comm_trm_val_def_defs z x)).
+      inversion Hlc as [Hlc_ec Hlc_trm].
       inversions Hlc_ec. specialize (H7 z).
       apply (lc_opening 1 x) in H7. unfold open_trm in H7. rewrite H7.
       assert (z \notin L0) by auto.
-      specialize (H1 z H4).
+      specialize (H2 z H4).
       eapply weaken_rules; eauto.
     + eapply IHHt with (L:=L \u (dom G)); auto. intros.
       assert (x \notin L) by auto.
-      specialize (H1 x H2).
+      specialize (H2 x H1).
       eapply narrow_typing; eauto. apply~ subenv_last.
 Qed.
 
 Lemma progress_red: forall G e t T,
-    inert G ->
     ty_ec_trm G e t T ->
     (normal_form e t \/ exists e' t', e / t |-> e' / t').
 Proof.
-  introv Hi Ht.
+  introv Ht.
   destruct e.
-  - inversions Ht. rename H0 into Hwf. rename H2 into Ht.
+  - inversions Ht.
+    rename H0 into Hin. rename H1 into Hwf. rename H3 into Ht.
     dependent induction Ht; try solve [left; auto].
-    * destruct (canonical_forms_fun Hi Hwf Ht1) as [L [T' [t [Bis [Hsub Hty]]]]].
+    * destruct (canonical_forms_fun Hin Hwf Ht1) as [L [T' [t [Bis [Hsub Hty]]]]].
       right. repeat eexists. apply* red_apply.
-    * destruct (canonical_forms_obj Hi Hwf Ht) as [S [ds [t [Bis [Has Ty]]]]].
+    * destruct (canonical_forms_obj Hin Hwf Ht) as [S [ds [t [Bis [Has Ty]]]]].
       right. repeat eexists. apply* red_project.
     * right. exists (e_term s u) t.
       apply red_congruence_let.
-    * specialize (IHHt Hi) as [IH | [t' [s' Hred]]].
+    * specialize (IHHt Hin) as [IH | [t' [s' Hred]]].
       + assumption.
       + left. assumption.
       + right. exists t' s'. assumption.
-  - inversions Ht. clear H6.
-    rename H1 into Hwf. rename H3 into Ht.
+  - inversions Ht. clear H7.
+    rename H1 into Hin. rename H2 into Hwf. rename H4 into Ht.
     dependent induction Ht; right.
     * repeat eexists; apply red_let_var.
     * pick_fresh x. repeat eexists; apply red_congruence_val with (x:=x); auto.
-    * destruct (canonical_forms_fun Hi Hwf Ht1) as [L' [T' [t [Bis [Hsub Hty]]]]].
+    * destruct (canonical_forms_fun Hin Hwf Ht1) as [L' [T' [t [Bis [Hsub Hty]]]]].
       repeat eexists. apply* red_apply.
     * pick_fresh x. repeat eexists; apply red_congruence_val with (x:=x); auto.
-    * destruct (canonical_forms_obj Hi Hwf Ht) as [S [ds [t [Bis [Has Ty]]]]].
+    * destruct (canonical_forms_obj Hin Hwf Ht) as [S [ds [t [Bis [Has Ty]]]]].
       repeat eexists. apply* red_project.
     * repeat eexists; apply red_let_let.
     * repeat eexists; apply red_let_var.
     * repeat eexists; apply red_let_var.
     * repeat eexists; apply red_let_var.
-    * specialize (IHHt Hi) as [IH | [t' [s' Hred]]]; eauto.
+    * specialize (IHHt Hin) as [IH | [t' [s' Hred]]]; eauto.
       inversion IH.
 Qed.
 
 Lemma progress: forall G e t T,
-    inert G ->
     lc_term e t ->
     ty_ec_trm G e t T ->
     (normal_form e t \/
@@ -256,7 +255,7 @@ Lemma progress: forall G e t T,
        e / t |-> e' / t' /\
        lc_term e' t').
 Proof.
-  introv Hi Hlc Ht. destruct (progress_red Hi Ht).
+  introv Hlc Ht. destruct (progress_red Ht).
   - left~.
   - destruct H as [e' [t' Hred']]. right. exists e' t'. split~.
     eapply red_preserves_lc; eauto.
